{
 "cells": [
  {
   "cell_type": "markdown",
   "metadata": {},
   "source": [
    "### 01 Summation Notation\n",
    "Enter closed-form expressions, without summation notation, in terms of the variables given in each question."
   ]
  },
  {
   "cell_type": "markdown",
   "metadata": {},
   "source": [
    "### Question 01\n",
    "$$\n",
    "\\sum_{i=0}^{N} 1\n",
    "$$\n",
    "\n",
    "**Explanation**\n",
    "To evaluate the summation $\\sum_{i=0}^{N} 1$, we can observe that the term being summed is always equal to 1. Since we are summing the term 1 for each value of $i$ from 0 to \\(N\\), the result will be the total number of terms in the summation, which is \\(N+1\\).\n",
    "\n",
    "Therefore, the simplified form of the given summation is:\n",
    "$$\n",
    "\\sum_{i=0}^{N} 1 = N+1\n",
    "$$\n"
   ]
  },
  {
   "cell_type": "markdown",
   "metadata": {},
   "source": [
    "### Question 02\n",
    "$$\n",
    "\\sum _{k=1}^{K} \\sum _{t=1}^{T} 1\n",
    "$$\n",
    "\n",
    "**Explanation**\n",
    "To evaluate the given double summation, we can observe that the term being summed is always equal to 1. Since we are summing the term 1 for each value of \\(k\\) from 1 to \\(K\\) and for each value of \\(t\\) from 1 to \\(T\\), the result will be the total number of terms in the summation, which is $K \\times T$.\n",
    "\n",
    "Therefore, the simplified form of the given double summation is:\n",
    "\n",
    "$$\n",
    "\\sum _{k=1}^{K} \\sum _{t=1}^{T} 1 = K \\times T\n",
    "$$"
   ]
  },
  {
   "cell_type": "markdown",
   "metadata": {},
   "source": [
    "### Question 03\n",
    "\n",
    "$$\n",
    "\\sum_{k=1}^{K} \\sum_{t=1}^{T} 0.5^k\n",
    "$$\n",
    "\n",
    "**Explnation**\n",
    "This expression consists of two summations:\n",
    "\n",
    "1. The outer summation, indexed by \\( k \\), running from 1 to \\( K \\).\n",
    "2. The inner summation, indexed by \\( t \\), running from 1 to \\( T \\).\n",
    "\n",
    "The term being summed is \\( 0.5^k \\), which depends only on the outer index \\( k \\).\n",
    "\n",
    "Here's the step-by-step breakdown:\n",
    "\n",
    "1. **Inner Summation**: The inner summation is over \\( t \\), but the term \\( 0.5^k \\) does not depend on \\( t \\). This means that for each fixed \\( k \\), the inner summation is just \\( T \\) times \\( 0.5^k \\).\n",
    "\n",
    "   $$\n",
    "   \\sum_{t=1}^{T} 0.5^k = T \\cdot 0.5^k\n",
    "   $$\n",
    "\n",
    "2. **Outer Summation**: Now, we sum the result of the inner summation over \\( k \\) from 1 to \\( K \\).\n",
    "\n",
    "   $$\n",
    "   \\sum_{k=1}^{K} T \\cdot 0.5^k\n",
    "   $$\n",
    "\n",
    "   Since \\( T \\) is a constant with respect to \\( k \\), it can be factored out:\n",
    "\n",
    "   $$\n",
    "   T \\cdot \\sum_{k=1}^{K} 0.5^k\n",
    "   $$\n",
    "\n",
    "3. **Geometric Series**: The summation \\( \\sum\\_{k=1}^{K} 0.5^k \\) is a geometric series with the first term \\( a = 0.5 \\) and common ratio \\( r = 0.5 \\).\n",
    "\n",
    "   The sum of the first \\( K \\) terms of a geometric series is given by:\n",
    "\n",
    "   $$\n",
    "   \\sum_{k=1}^{K} r^k = r \\frac{1 - r^K}{1 - r}\n",
    "   $$\n",
    "\n",
    "   Plugging in \\( r = 0.5 \\):\n",
    "\n",
    "   $$\n",
    "   \\sum_{k=1}^{K} 0.5^k = 0.5 \\frac{1 - 0.5^K}{1 - 0.5} = 0.5 \\frac{1 - 0.5^K}{0.5} = 1 - 0.5^K\n",
    "   $$\n",
    "\n",
    "4. **Combining Results**: Substitute this result back into our expression:\n",
    "\n",
    "   $$\n",
    "   T \\cdot (1 - 0.5^K)\n",
    "   $$\n",
    "\n",
    "So, the double summation simplifies to:\n",
    "\n",
    "$$\n",
    "\\sum_{k=1}^{K} \\sum_{t=1}^{T} 0.5^k = T \\cdot (1 - 0.5^K)\n",
    "$$\n",
    "\n",
    "This is the simplified form of the given double summation."
   ]
  },
  {
   "cell_type": "markdown",
   "metadata": {},
   "source": [
    "### Question 04\n",
    "\n",
    "$$ \\sum_{k=1}^{\\infty} \\sum_{t=1}^{T} 0.5^k $$\n",
    "\n",
    "**Explanation**\n",
    "This expression is similar to the previous one, with the difference that the outer summation now runs to infinity (\\(\\infty\\)) instead of a finite upper limit \\(K\\). Let's break it down:\n",
    "\n",
    "1. **Inner Summation**: The inner summation is still over \\( t \\), but the term \\( 0.5^k \\) does not depend on \\( t \\). This means that for each fixed \\( k \\), the inner summation is just \\( T \\) times \\( 0.5^k \\):\n",
    "\n",
    "   $$\n",
    "   \\sum_{t=1}^{T} 0.5^k = T \\cdot 0.5^k\n",
    "   $$\n",
    "\n",
    "2. **Outer Summation**: Now, we sum the result of the inner summation over \\( k \\) from 1 to infinity:\n",
    "\n",
    "   $$\n",
    "   \\sum_{k=1}^{\\infty} T \\cdot 0.5^k\n",
    "   $$\n",
    "\n",
    "   Since \\( T \\) is a constant with respect to \\( k \\), it can be factored out:\n",
    "\n",
    "   $$\n",
    "   T \\cdot \\sum_{k=1}^{\\infty} 0.5^k\n",
    "   $$\n",
    "\n",
    "3. **Geometric Series**: The summation \\( \\sum_{k=1}^{\\infty} 0.5^k \\) is an infinite geometric series with the first term \\( a = 0.5 \\) and common ratio \\( r = 0.5 \\). The sum of an infinite geometric series \\( \\sum_{k=0}^{\\infty} ar^k \\) is given by:\n",
    "\n",
    "   $$\n",
    "   \\sum_{k=1}^{\\infty} r^k = \\frac{r}{1 - r}\n",
    "   $$\n",
    "\n",
    "   Plugging in \\( r = 0.5 \\):\n",
    "\n",
    "   $$\n",
    "   \\sum_{k=1}^{\\infty} 0.5^k = \\frac{0.5}{1 - 0.5} = \\frac{0.5}{0.5} = 1\n",
    "   $$\n",
    "\n",
    "4. **Combining Results**: Substitute this result back into our expression:\n",
    "\n",
    "   $$\n",
    "   T \\cdot 1 = T\n",
    "   $$\n",
    "\n",
    "So, the double summation simplifies to:\n",
    "\n",
    "$$\n",
    "\\sum_{k=1}^{\\infty} \\sum_{t=1}^{T} 0.5^k = T\n",
    "$$\n",
    "\n",
    "This is the simplified form of the given double summation."
   ]
  }
 ],
 "metadata": {
  "language_info": {
   "name": "python"
  }
 },
 "nbformat": 4,
 "nbformat_minor": 2
}
